\documentclass{article}
\usepackage{bm}
\usepackage{amsmath}
\usepackage{amsthm}
\usepackage{url}
\usepackage{amssymb}
\newtheorem{theorem}{Theorem}
\newtheorem{lemma}{Lemma}
\newtheorem{corollary}{Corollary}
\DeclareMathOperator{\E}{\mathbb{E}}
\title{Proofs for semi-supervised SBM}
\begin{document}
\maketitle
\begin{lemma}
Let $Z_{i2}$ follows Bernoulli distribution with parameter $q=\frac{\beta \log n }{n}$.
Let $Z_{i1} \sim Bern(p)$ with $p=\frac{\alpha \log n }{n}$. $Z_{i2}$ are i.i.d. for $i=1,\dots, n$.
The same is true for $Z_{i1}$. $\beta < \alpha$.
We then have $P(\sum_{i=1}^{n} (Z_{i2} - Z_{i1}) \geq  D \log n) \leq n^{-C}$
where $C=\frac{3(\alpha - \beta + D)^2}{2(4\alpha + 2\beta + D)} + O(\log n /n)$.
\end{lemma}
\begin{proof}
	Let $X_i = Z_{i2} - \frac{\beta \log n }{n}, X_{i+n} = \frac{\alpha \log n }{n} - Z_{i1}$.
	$X_i$ are zero means and $|X_i| \leq 1 + O(\frac{\log n}{n})$.
	Then $\sum_{i=1}^{n} (Z_{i2} - Z_{i1}) = \sum_{i=1}^{2n} X_{i} - (\alpha - \beta)\log n $.
	Then $\sum_{i=1}^{n} (Z_{i2} - Z_{i1}) \geq D \log n \iff \sum_{i=1}^{2n} X_{i} \geq (D + \alpha - \beta)\log n$.
	$\sum_{i=1}^{2n} E[X_i^2] = (\alpha + \beta)\log n + O(\frac{\log^2 n}{n})$.
	By Bernstein's inequality, we have
	$$
	P(\sum_{i=1}^{2n} X_{i}  \geq t) \leq \exp(-\frac{1/2 t^2}{\sum_{i=1}^{2n} E[X_i^2] + \frac{1}{3}(1+O(\log n /n))t})
	$$
	Let $t=(D + \alpha - \beta)\log n$.
	\begin{align}
	\frac{1/2 t^2}{\sum_{i=1}^{2n} E[X_i^2] + \frac{1}{3}t} & 
	= \frac{1/2(D + \alpha - \beta)^2\log^2 n}{(\alpha + \beta)\log n + O(\frac{\log^2 n}{n}) + 1/3(D + \alpha - \beta)\log n } \\
	 & =\frac{3/2(D + \alpha - \beta)^2\log n}{O(\frac{\log n}{n}) + (D + 4\alpha - 2\beta) }
	\end{align}
\end{proof}
Notation: $f(n)\dot{=} g(n) \iff \lim_{n\to \infty} \frac{1}{n} \log \frac{f(n)}{g(n)} = 1$.
\begin{lemma}\label{lem:coupled}
	Suppose $x_i$ is i.i.d. sampled from $p_1$ and $z_i$ is i.i.d. sampled from $Bern(p)$.
	$p > q$
Let $A := \frac{1}{n}\sum_{i=1}^n \log \frac{p_0(x_i)}{p_1(x_i)} \geq \frac{1}{n} \sum_{i=1}(z_i \log\frac{p}{q} +(1-z_i) \frac{\log(1-p)}{\log(1-q)}))$.
Show that $P(A) \dot{=} \exp(-n C)$.
\end{lemma}
\begin{proof}
	To apply Sanov's theorem, we treat $(x_i, z_i)$ jointly sampled from $\mathcal{X} \times \mathcal{Z}$
	and the constraint is 
	\begin{equation}\label{eq:fxz}	
	\frac{1}{n} \sum_{i=1}^n f(x_i, z_i) \geq 0
	\end{equation}	
	where
	$$
	f(x, z) = \log\frac{p_0(x)}{p_1(x)} + z \log\frac{q}{p} + (1-z) \log \frac{1-q}{1-p}
	$$
	Then by Sanov's theorem, we have $C = D(p^*(x,z)|| p_1(x)Bern(p))$
	where $p^*(x,z)$ is the minimizer for $D(p(x,z)|| p_1(x)Bern(p))$ subjected to
	\eqref{eq:fxz}.
	We can rewrite \eqref{eq:fxz} in probability form:
	\begin{equation}\label{eq:probxz}
	\sum_{x\in \mathcal{X}} p(x) \log\frac{p_0(x)}{p_1(x)} + \sum_{z \in \{0,1\}} p(z) \log\frac{p_{Bq}(z)}{p_{Bp}(z)} \geq 0
	\end{equation}
	where $p(x), p(z)$ are the marginal probability mass function.
	Using Lagrange's method, we can get
	\begin{equation}
	p^*(x,z) = C_1 p_0^{\lambda}(x)p_1^{1-\lambda}(x) \cdot C_2 p_{Bq}^{\lambda}(z)p_{Bp}^{1-\lambda}(z)
	\end{equation}
	where $\frac{1}{C_1} = \sum_{x\in\mathcal{X}}p_0^{\lambda}(x)p_1^{1-\lambda}(x) $
	and $\frac{1}{C_2} = \sum_{z\in \{0,1\}} p_{Bq}^{\lambda}(z)p_{Bp}^{1-\lambda}(z)$
	The parameter $\lambda$ is solved by letting the left hand of \eqref{eq:probxz} takes zero.
	That is:
	\begin{equation}\label{eq:constraint}
	C_1 \sum_{x\in \mathcal{X}} p_0^{\lambda}(x)p_1^{1-\lambda}(x)\log\frac{p_0(x)}{p_1(x)} + C_2[p^{1-\lambda}q^{\lambda}\log\frac{q}{p} +
	(1-p)^{1-\lambda}(1-q)^{\lambda}\log\frac{1-q}{1-p} ] = 0
	\end{equation}
	On the other hand,
	\begin{align*}
	C(k) & = D(p(x)|| p_1(x)) + D(p(z) || Bern(p)) \\
	& = C_1\sum_{x\in \mathcal{X}} p_0^{\lambda}(x)p_1^{1-\lambda}(x)\log\frac{C_1  p_0^{\lambda}(x)p_1^{1-\lambda}(x)}{p_1(x)}  \\
	& + C_2[p^{1-\lambda}q^{\lambda}\log\frac{C_2 p^{1-\lambda}q^{\lambda}}{p} +
	(1-p)^{1-\lambda}(1-q)^{\lambda}\log\frac{C_2(1-p)^{1-\lambda}(1-q)^{\lambda}}{(1-p)} ] 
	\end{align*}
	Using \eqref{eq:constraint}, we can simplify $C$ as
	\begin{equation}
	C  =  \log  C_1 + \log C_2
	\end{equation}
	Using $p_0^{\lambda} p_1^{1-\lambda} \leq \lambda p_0 + (1-\lambda) p_1$ we can get $C_1 > 1, C_2 > 1$.

\end{proof}
\begin{corollary}\label{cor:xz}
	Let $p_0 \sim Bern(p), p_1 \sim Bern(q)$ in Lemma \ref{lem:coupled}. Then the region $A$ can be simplified as $\sum_{i=1}^n (x_i - z_i) \geq 0$,
	where $x_i \in Bern(q), z_i \in Bern(p)$ and both are i.i.d. sampled. We can compute $\lambda = \frac{1}{2}$ and the error exponent
	$C = -2\log(\sqrt{pq} + \sqrt{(1-p)(1-q)})$. Below we give another way to prove that $P(A) \dot{=} \exp(-nC)$.
\end{corollary}
\begin{proof}
	We use Chernoff inequality to give a tight upper bound.
	$P(\sum_{i=1}^n (x_i - z_i) \geq 0) \leq \E[\exp(\beta \sum_{i=1}^n (x_i - z_i))]$ where $\beta > 0$.
	$\E[\exp(\beta \sum_{i=1}^n (x_i - z_i))] = (1-q+q e^{\beta})^n(1-p+p e^{-\beta})^n$. Let
	$g(\beta)  = (1-q+q e^{\beta})(1-p+p e^{-\beta})$. $g(0) = 1$ and when $\beta$ is very small,
	$g(\beta) = 1 + (q-p) \beta + o(\beta)$. Therefore, we can choose a proper $\beta$ such that $g(\beta) < 1$.
	Since $\beta$ can take any positive value, now we compute the minimum value of $g(\beta)$ instead.
	the optimal $\beta^*$ satisfies $e^{2\beta} = \frac{(1-q)p}{(1-p)q}$. Now we compute $C' = -\log g(\beta^*) = C$.
	Therefore, $P(A) \leq \exp(-nC)$.
	
	To simplify our discussion, let $X_n = \sum_{i=1}^n X_i, Z_n = \sum_{i=1}^n Z_i$. We have $X_n \sim Binomial(n, q),
	Z_n \sim Binomial(n, p)$ and $X_n, Z_n$ are independent.
	
	On the other hand $P(A) = \sum_{j=1}^n\sum_{k=0}^j P(X_n = j)P(Z_n = k)$.
	We choose a proper $j,k$ such that $P(X_n = j)P(Z_n = k)$ is maximized.
	Since we observe $P(X_n - Z_n = r)$ decreases as $r$ increase ($r\geq 0$).
	The maximum value is taken when $j=k$. On the other hand,
	we should choose:
	$$
	k = n \frac{\sqrt{pq}}{\sqrt{pq} + \sqrt{(1-p)(1-q)}}
	$$
	We have
$$
		P(X_n = k)P(Z_n = k) = \binom{n}{k}^2 p^k (1-p)^{n-k}q^k(1-q)^{n-k}
$$
We will use the inequality $\binom{n}{k} \geq \frac{1}{n+1}\exp(nH(k/n))$.
Then
$$
\log P(X_n = k)P(Z_n = k) \geq -2\log(n+1) + 2n \log(\sqrt{pq} + \sqrt{(1-p)(1-q)})
$$
Therefore, $\log P(A) \geq \log P(X_n = k)P(Z_n = k) \geq -2\log(n+1) + 2n \log(\sqrt{pq} + \sqrt{(1-p)(1-q)})$.
That is $P(A) \geq \frac{1}{(n+1)^2}\exp(-nC)$.
The polynomial term is neglectable compared with the exponential term.
\end{proof}
\begin{lemma}\label{lem:nk}
	$\binom{n}{k} < (\frac{ne}{k})^k$
\end{lemma}
\begin{proof}
	$\binom{n}{k} = \frac{n!}{(n-k)!k!} < \frac{n^k}{k!}$.
	Since $e^z = \sum_{k=0}^{\infty} \frac{z^k}{k!} > \frac{z^k}{k!}$,
	let $z=k$ we have $e^k > \frac{k^k}{k!}$.
	Therefore, $\frac{1}{k!} < \frac{e^k}{k^k}$.
	As a result, $\binom{n}{k}  < \frac{n^k}{k!} < \frac{n^k e^k}{k^k}
	= (\frac{ne}{k})^k$
\end{proof}
\begin{theorem}\label{thm:2pq}
	For a $\textrm{SBM}(n,2,p, q)$ with $p,q$ as constant, $p > q$. The
	exact recovery error decreases in $\exp(-n (C + o(1)))$
	where $C = -2\log(\sqrt{pq} + \sqrt{(1-p)(1-q)})$.
\end{theorem}
\begin{proof}
	We use maximum likelihood estimation method, let $F$ be the event of the maximum likelihood estimator not coinciding with the ground truth. 
    
    We use $P_n^{(k)}$ to denote the event when there are $k$ pairs wrongly classified. Due to the symmetric property of the problem, $1\leq k \leq \frac{n}{4}$.
    $P_n^{(k)}$ happens when the probability of one $k$ mis-classified configuration has larger probability than that of the ground truth. 
	
	Therefore, we consider one configuration of $k=1$. Let event $A$ be the ground truth and $A_1$ be our chosen event:
	\begin{align*}
	A: & y_1 = 1, y_2 = 0, y_3 = 1, y_4 = 0, \dots, y_{n-1} = 1, y_n = 0 \\
	A_1: & y_1 = 0, y_2 = 1, y_3 = 1, y_4 = 0, \dots, y_{n-1} = 1, y_n = 0 \\	
	\end{align*}
	Then if $P(A) < P(A_1)$, event $F$ will happen. Therefore, we use $P(P(A) < P(A_1))$ as the lower bound of $P(F)$.
	By simplification we get $P(\sum_{i=1}^{n-2} (x_i - z_i) \geq 0) \dot{=} \exp{-nC}$ where $x_i, z_i$ are the same with Corollary \ref{cor:xz}.
	
	For the upper bound, we next show that 
	\begin{equation}
	P(F) \leq \frac{en^2}{4} \exp(-nC).
	\end{equation}
	where $e$ is the natural logarithm number.
	
	When $F$ happens, then $P(A)$ is not the maximum value, there must exists one configuration $P(A') > P(A)$, by the union bound we have:
	\begin{equation}\label{eq:outsidelemmaboundpf5_IT_ub}
	P(F) \leq \sum_{A'} P(P(A') > P(A))
	\end{equation}
	We can classify the right hand by grouping according to the index $k$. That is
	\begin{equation}\label{eq:with14epsilon_14}
	\sum_{A'} P(P(A') > P(A)) = \sum_{k=1}^{n/4} P_{n}^{(k)}
	\end{equation}
	where $P_{n}^{(k)} = \binom{n/2}{k}^2 P(P(A_k) > P(A))$ and $A_k$ is one configuration with $k$ pairs mis-classified.
	Similar to the case $k=1$ we can compute $P(P(A_k) > P(A)) = P(\sum_{i=1}^{k(n-2k)} (x_i - z_i) \geq 0)\dot{=} \exp(-k(n-2k)C)$.
	
	Combining (\ref{eq:outsidelemmaboundpf5_IT_ub}) and (\ref{eq:with14epsilon_14}), we have
	\begin{equation}
	P(F) \leq \sum_{k=1}^{n/4} \binom{n/2}{k}^2 \exp(-k(n-2k)C)
	\end{equation}
	Using the inequality from Lemma \ref{lem:nk}, we have
	\begin{equation}
		P(F) \leq \sum_{k=1}^{n/4} \exp(-nf(k))
	\end{equation}
	where $f(k)= \frac{2k}{n}\log\frac{2k}{ne} + k(1-\frac{2k}{n})C$.
	By computing $f'(x)= \frac{2}{n} \log \frac{2x}{n} + C - \frac{4Cx}{n}$, $1\leq x \leq \frac{n}{4}$.
	$f'(1) > 0 , f'(\frac{n}{4}) < 0$. Therefore, $f(x)$ increases first and decreases in the interval $[1, \frac{n}{4}]$.
	Comparing $f(1)$ and $f(\frac{n}{4})$ we have $f(1) < f(\frac{n}{4})$. Therefore, $f(k) \geq f(1)$ for $1\leq k \leq \frac{n}{4}$.
	\begin{equation}
	P(F) \leq \frac{n}{4}\exp(-nf(1)) = \exp(-n (C+g(n)))
	\end{equation}
	where $g(n) = -\frac{1}{n}(\log (n/4) + 2 C - 2 \log (2/ne)) = o(1)$
\end{proof}
\begin{theorem}
	In $\textrm{SBM}(n, 2, p, q)$ where $p,q$ are constant, each node has further $n$ observations based on its label.
	That is $ x_{ij} \sim p_{y_i}$ where $y_i = 0 $ or $y_i = 1$. $D(p_0 || p_1) > 0$. Then generally we will have
	the exact recovery error decreases in $\exp(-nC')$. where $C'$ is a constant irreverent with $n$.
\end{theorem}
\begin{proof}
	The proof is similar with that of Theorem \ref{thm:2pq} and we have
	\begin{equation}
	C' = -2 \log(\sqrt{pq} + \sqrt{(1-p)(1-q)}) - 2 \log \sum_{x\in \mathcal{X}} \sqrt{p_0(x)p_1(x)}
	\end{equation}
\end{proof}
\end{document}