\documentclass{article}
\usepackage{amsmath}
\usepackage{amssymb}
\usepackage{amsthm}
\def\E{\mathbb{E}}
\DeclareMathOperator{\tr}{Tr}
\title{SDP ands its duality}
\begin{document}
\maketitle
\section{Lagrange Dual Theory}
See \cite{dual}. This theory can be used to get the dual problem for LP and SDP.
First consider
\begin{align*}
\min\, & c^T x \\
s.t. \,& Ax = b \\
&x \geq 0
\end{align*}
We write the Lagrange function as
$L(x,y) = c^T x - y^T(Ax-b) = (c - A^Ty)^Tx + b^T y$.
We minimize $L(x,y)$ subjected to $x \geq 0$. The domain of definition for the dual function should exclude
those $y$ such that $-\infty = L(x,y)$. Therefore, we should have $c-A^Ty \geq 0$ and
the dual problem becomes:
\begin{align*}
\max\, & b^T y \\
s.t. \,& A^T y \leq c
\end{align*}
The same can be said about SDP problem. Following 12.2 of \cite{sdp} we consider the primal problem as:
\begin{align*}
\min\,& C \cdot X \\
s.t. \,& A_i \cdot X = b_i, i=1,\dots, m \\
& X \succeq 0
\end{align*}
The inner product of two symmetric matrix is defined by $A\cdot B = \tr(A^TB) = \sum_{i,j=1}^n A_{ij}B_{ij}$.
The norm associated with such inner product is Frobenius norm.

Similar to the deduction of LDP problem, we consider $L(X,y)= C\cdot X - \sum_{i=1}^m y_i (A_i \cdot X - b_i)
=(C-\sum_{i=1}^m y_i A_i)\cdot X + \sum_{i=1}^m b_i y_i$.
If $C-\sum_{i=1}^m y_i A_i \not\in S_n^+$, then we can find vector $z$ such that 
$z^T(C-\sum_{i=1}^m y_i A_i)z = (C-\sum_{i=1}^m y_i A_i) \cdot zz^T < 0$ Let $X=\lambda zz^T \in S_n^+$
we can make $L(X,y) \to -\infty$. Therefore, $C-\sum_{i=1}^m y_i A_i \succeq 0$.
And we get the dual problem of SDP:
\begin{align*}
\max\,&\sum_{i=1}^m b_i y_i \\
s.t.\,& \sum_{i=1}^m y_i A_i \preceq C
\end{align*}
\begin{thebibliography}{9}
	\bibitem{dual} https://de.wikipedia.org/wiki/Lagrange-DualitÃ¤t
	\bibitem{sdp} https://www.cs.cmu.edu/afs/cs.cmu.edu/academic/class/15859-f11/www/notes/lecture12.pdf
\end{thebibliography}
\end{document}
